coq/NumberParsing.v
@@ -1,0 +1,102 @@
+Require Import Koika.Frontend.
+
+(* Inductive parsed_bit_list :=
+| Nil_bit_list
+| Cons_bit_list : forall (b: bool) (bs: parsed_bit_list), parsed_bit_list. *)
+
+Print Decimal.uint.
+
+Import Decimal.
+
+Fixpoint sz_of_dec_uint (d : Decimal.uint) :=
+  match d with
+  | Nil => 0
+  | D0 d | D1 d | D2 d | D3 d | D4 d
+  | D5 d | D6 d | D7 d | D8 d | D9 d
+    => 1 + (sz_of_dec_uint d)
+  end.
+
+Definition sz_of_num_uint (n : Number.uint) :=
+  match n with
+  | Number.UIntDecimal d => sz_of_dec_uint d
+  | Number.UIntHexadecimal h => 0
+  end.
+
+(* Fixpoint bits_of_dec_uint (d: Decimal.uint) : option (Bits.bits (sz_of_dec_uint d)).
+  destruct d.
+  unfold sz_of_dec_uint. exact (Some Bits.nil).
+
+  unfold sz_of_dec_uint. exact (Some (@Bits.cons (sz_of_dec_uint d) false (bits_of_dec_uint d))).
+  all: exact None.
+Defined. *)
+
+(* Print bits_of_dec_uint. *)
+  
+
+Fixpoint bits_of_dec_uint (d: Decimal.uint) : option (Bits.bits (sz_of_dec_uint d)) :=
+    match d as d' return (option (Bits.bits (sz_of_dec_uint d'))) with
+    | Decimal.Nil => match sz_of_dec_uint d with _ => Some Bits.nil end
+    | Decimal.D0 d => option_map (fun d' => Bits.snoc false d') (bits_of_dec_uint d)
+    | Decimal.D1 d => option_map (fun d' => Bits.snoc true d') (bits_of_dec_uint d)
+    | _ => None
+    end.
+
+Definition bits_of_num_uint (d: Number.uint) : option (Bits.bits (sz_of_num_uint d)) :=
+  match d with
+  | Number.UIntDecimal d =>
+    bits_of_dec_uint d
+  | Number.UIntHexadecimal h => None
+  end.
+
+Compute (bits_of_num_uint 01101%uint).
+(* 
+Fixpoint decode_bitstring_from_bits (sz: nat) (bs: parsed_bit_list) : option (bits sz) :=
+  match sz with
+  | 0 =>
+    match bs with
+    | Nil_bit_list => Some Ob
+    | _ => None
+    end
+  | S sz =>
+    let/opt2 hd, bs :=
+       match bs with
+       | Nil_bit_list => Some (false, bs)
+       | Cons_bit_list hd bs => Some (hd, bs)
+       end in
+    let/opt tl :=
+       decode_bitstring_from_bits sz bs in
+    Some tl~hd
+  end. *)
+
+Inductive NumberParsingError :=
+  NumberParsingError_OutOfBounds.
+
+Definition must_bits {sz} (o: option (bits sz)) : if o then bits sz else NumberParsingError :=
+  match o with
+  | Some bs => bs
+  | None => NumberParsingError_OutOfBounds
+  end.
+
+Fixpoint pr' {sz} (b : bits sz) : Decimal.uint :=
+  match sz as n return (bits n -> Decimal.uint) with
+  | 0 => fun _ => Decimal.Nil
+  | S _ => fun b' => if (Bits.hd b')
+    then Decimal.D1 (pr' (Bits.tl b'))
+    else Decimal.D0 (pr' (Bits.tl b'))
+  end b.
+
+Definition pr {sz} (bl : bits sz) : Number.uint :=
+  Number.UIntDecimal (pr' bl).
+
+
+
+Declare Scope bitstrings_scope.
+Delimit Scope bitstrings_scope with bitstrings.
+(* Number Notation bits decode_bits_from_parsed_uint pr : bitstrings_scope. *)
+(* Notation "'0b' num ':b' sz" :=
+  (tc_compute (must_bits (decode_bitstring_from_bits sz num%bitstrings) : bits sz))
+    (at level 2, no associativity).
+
+Check 0110101%bitstrings.
+
+Check (0b11:b32).                 FIXME remove type annotation *)
