coq/Theorems/CompactLogsCorrectness.v
@@ -1,0 +1,187 @@
+Require Koika.CompactLogs.
+Require Koika.CompactSemantics.
+Require Koika.Logs.
+Require Koika.TypedSyntax.
+Require Koika.TypedSemantics.
+Require Import Koika.FiniteType.
+Require Import Koika.Types.
+Require Import Koika.Environments.
+
+Section CompactEquality.
+  Context {reg_t ext_fn_t var_t pos_t fn_name_t: Type}.
+  Context {ft : FiniteType reg_t}.
+  Context {tau : type}.
+  Context {sig : tsig var_t}.
+
+  Context {REnv: Env reg_t}.
+
+  Context {R : reg_t -> type}.
+  Context {sigma : (ext_fn_t -> ExternalSignature)}.
+
+  Context {r : (forall reg : reg_t, R reg)}.
+
+  Definition tcontext (sig: tsig var_t) :=
+    context (fun k_tau => type_denote (snd k_tau)) sig.
+  Context {Gamma : tcontext sig}.
+
+  Context {a : TypedSyntax.action pos_t var_t fn_name_t R sigma sig tau}.
+
+  Context {sigma_denote : (forall fn: ext_fn_t, Sig_denote (sigma fn))}.
+
+  Lemma Logs_latest_write_empty :
+    forall idx : reg_t,
+    @Logs.latest_write _ R REnv Logs.log_empty idx = None.
+  Proof.
+    intros.
+    unfold Logs.latest_write, Logs.log_find, Logs.log_empty.
+    rewrite getenv_create.
+    reflexivity.
+  Defined.
+
+  Lemma Logs_commit_update_empty :
+    forall env : REnv.(env_t) R,
+    Logs.commit_update env Logs.log_empty = env.
+  Proof.
+    intros.
+    unfold Logs.commit_update.
+    apply equiv_eq.
+    unfold equiv.
+    intros.
+    rewrite getenv_create.
+    rewrite Logs_latest_write_empty.
+    reflexivity.
+  Defined.
+
+  Lemma CompactLogs_commit_update_empty :
+    forall env : REnv.(env_t) R,
+    CompactLogs.commit_update env CompactLogs.log_empty = env.
+  Proof.
+    intros.
+    unfold CompactLogs.commit_update.
+    apply equiv_eq.
+    unfold equiv.
+    intro.
+    rewrite getenv_create.
+    unfold CompactLogs.log_empty.
+    rewrite getenv_create.
+    reflexivity.
+  Defined.
+
+  Disable Notation "'let/opt' v1 ':=' expr 'in' body".
+  Disable Notation "'let/opt2' v1 ',' v2 ':=' expr 'in' body".
+
+
+  Lemma opt_bind_none {A B} {f : A -> option B} :
+    forall x : option A,
+    x = None ->
+    opt_bind x f = None.
+  Proof. intros x H. rewrite H. reflexivity. Defined.
+
+  Lemma compact_typed_eq_abort {env : REnv.(env_t) R} :
+
+    (CompactSemantics.interp_action env sigma_denote Gamma CompactLogs.log_empty CompactLogs.log_empty a) = None
+    <->
+    (TypedSemantics.interp_action env sigma_denote Gamma Logs.log_empty Logs.log_empty a) = None.
+  Proof.
+    induction a.
+    - simpl; split; (reflexivity + discriminate).
+    - simpl; split; (reflexivity + discriminate).
+    - simpl; split; (reflexivity + discriminate).
+    - simpl.
+      repeat match goal with
+      | |- context [let '(_,_) := ?x in _] => destruct x
+      | |- context [opt_bind ?x] => destruct x eqn:?H; simpl
+      end.
+      + split; (reflexivity + discriminate).
+      + split; try (reflexivity + discriminate).
+        specialize (IHa0 Gamma a0). rewrite H in IHa0. rewrite H0 in IHa0. destruct IHa0. specialize (H2 eq_refl). discriminate.
+      + split; try (reflexivity + discriminate).
+        specialize (IHa0 Gamma a0). rewrite H in IHa0. rewrite H0 in IHa0. destruct IHa0. specialize (H1 eq_refl). discriminate.
+      + split; (reflexivity + discriminate).
+    - simpl.
+      repeat match goal with
+      | |- context [let '(_,_) := ?x in _] => destruct x
+      | |- context [opt_bind ?x] => destruct x eqn:?H; simpl
+      end.
+      unfold opt_bind.
+      repeat match goal with
+      |- context [match ?x with | _ => _ end] => destruct x eqn:?
+      end.
+      all: split.
+      all: try discriminate; try reflexivity.
+      specialize (IHa0 Gamma a0).
+      destruct IHa0.
+      set (H0 Heqo0).
+      rewrite e in Heqo.
+      discriminate.
+      admit.
+    -
+
+      match goal with
+      |- context [match ?x with | Some _ => _ | None => _ end] => destruct x eqn:l
+      end.
+      + split. destruct p. destruct p.  discriminate.
+        destruct p0. destruct p0. discriminate.
+      +
+      specialize (IHa0 Gamma a0).
+       rewrite p in IHa0.
+      match goal with
+      |- context [match ?x with | _ => _ end] => destruct x
+      end.
+    rewrite ?opt_bind_none.  unfold opt_bind.
+    
+    split; discriminate.
+    - simpl.
+    split.
+
+
+
+  Lemma compact_typed_eq :
+    let env := REnv.(create) r in
+
+    option_map
+      (fun '(log,out,_) => (CompactLogs.commit_update env log, out))
+      (CompactSemantics.interp_action env sigma_denote Gamma CompactLogs.log_empty CompactLogs.log_empty a)
+    =
+    option_map
+      (fun '(log,out,_) => (Logs.commit_update env log, out))
+      (TypedSemantics.interp_action env sigma_denote Gamma Logs.log_empty Logs.log_empty a).
+  Proof.
+    intros.
+    induction a.
+    - unfold CompactSemantics.interp_action, TypedSemantics.interp_action, option_map. reflexivity.
+    - unfold CompactSemantics.interp_action, TypedSemantics.interp_action, option_map.
+        try rewrite CompactLogs_commit_update_empty;
+        try rewrite Logs_commit_update_empty;
+        reflexivity.
+    - unfold CompactSemantics.interp_action, TypedSemantics.interp_action, option_map.
+      try rewrite CompactLogs_commit_update_empty;
+      try rewrite Logs_commit_update_empty;
+      reflexivity.
+    - simpl.
+      Locate opt_bind.
+      unfold opt_bind.
+      unfold option_map.
+      unfold option_map in IHa0.
+      match goal with
+      |- context [match ?y with | Some x => (let '(p, Gamma0) := x in
+                                            let '(action_log, v) := p in
+                                            Some (action_log, Ob, creplace m v Gamma0))
+                                | None => None end] =>
+        fold (option_map (fun x => let '(p, Gamma0) := x in
+                                   let '(action_log, v) := p in
+                                   Some (action_log, Ob, creplace m v Gamma0)) y)
+      end.
+
+  Search (option).
+
+      unfold
+
+      apply IHa0.
+      assumption.
+      unfold option_map.
+      CompactSemantics.interp_action, TypedSemantics.interp_action, option_map.
+      try rewrite CompactLogs_commit_update_empty;
+      try rewrite Logs_commit_update_empty;
+      reflexivity.
+End CompactEquality.
